allocator/slabs bottom-up 11/n
add proper size_class vprop
- TODO: remove assume with vrefine vprops
- TODO: refine spec
- TODO: working extraction...

src/Slabs.fst
@@ -18,26 +18,12 @@ module L = FStar.List.Tot
 module SL = Selectors.LList
 module Temp = TempLock
 
-let array = Steel.ST.Array.array
-let ptr = Steel.ST.Array.ptr
 
 open FStar.Mul
 open Utils
-
-//TODO: should not be hardcoded
-let page_size = 4096ul
-let slab_max_number = 4096ul
-
-noextract
-let min_sc = 16
-noextract
-let max_sc = 64
-
-//TODO: second constraint should be relaxed
-//currently does not support size classes with <64 slots
-//that require a subtle loop to read only possible
-//corresponding slots in the bitmap
-let sc = x:U32.t{min_sc <= U32.v x /\ U32.v x <= max_sc}
+open Utils2
+open SlabsUtils
+open SizeClass
 
 let slab_region_len : U32.t = normalize_term (U32.mul page_size slab_max_number)
 unfold let slab_region
@@ -55,21 +41,9 @@ assume val get_slab_region (_:unit)
 assume val get_slab_md_region (_:unit)
   : slab_md_region
 
-let nb_slots (size_class: sc)
-  : Pure U32.t
-  (requires True)
-  (ensures fun r ->
-    U32.v r >= 1 /\
-    U32.v r <= 256
-  )
-  =
-  U32.div page_size size_class
-
 //TODO
 noextract
 let slab_md_bitmap_length = nb_slots (U32.uint_to_t min_sc)
-
-unfold let slab_metadata = r:array U64.t{A.length r = 4}
 
 #push-options "--z3rlimit 30"
 inline_for_extraction noextract
@@ -152,203 +126,6 @@ let get_free_slot (size_class: sc) (bitmap: slab_metadata)
   ) else (
     get_free_slot_aux size_class bitmap 0ul
   )
-
-#push-options "--z3rlimit 20"
-let slot_array (size_class: sc) (arr: array U8.t) (pos: U32.t)
-  : Pure (array U8.t)
-  (requires
-    U32.v pos < U32.v (nb_slots size_class) /\
-    A.length arr = U32.v page_size)
-  (ensures fun r ->
-    A.length r = U32.v size_class /\
-    same_base_array r arr /\
-    True)
-  =
-  let ptr = A.ptr_of arr in
-  let shift = U32.mul pos size_class in
-  assert (U32.v shift < A.length arr);
-  let ptr_shifted = A.ptr_shift ptr shift in
-  (| ptr_shifted, G.hide (U32.v size_class) |)
-#pop-options
-
-let array_slot (size_class: sc) (arr: array U8.t) (slot: array U8.t)
-  : Pure (G.erased int)
-  (requires same_base_array arr slot)
-  (ensures fun r -> True)
-  =
-  let ptr1 = A.ptr_of arr in
-  assert (A.offset ptr1 <= A.base_len (A.base ptr1));
-  let ptr2 = A.ptr_of slot in
-  assert (A.offset ptr2 <= A.base_len (A.base ptr2));
-  let offset_bytes = A.offset ptr2 - A.offset ptr1 in
-  let offset_slot = offset_bytes / (U32.v size_class) in
-  offset_slot
-
-let array_slot_slot_array_bij (size_class: sc) (arr: array U8.t) (pos: U32.t)
-  : Lemma
-  (requires
-    U32.v pos < U32.v (nb_slots size_class) /\
-    A.length arr = U32.v page_size)
-  (ensures (
-    let slot_as_array = slot_array size_class arr pos in
-    let slot_as_pos = array_slot size_class arr slot_as_array in
-    G.reveal slot_as_pos = U32.v pos))
-  =
-  let ptr = A.ptr_of arr in
-  let shift = U32.mul pos size_class in
-  assert (U32.v shift < A.length arr);
-  let ptr_shifted = A.ptr_shift ptr shift in
-  let slot_as_array = slot_array size_class arr pos in
-  assert (A.ptr_of slot_as_array == ptr_shifted);
-  let offset_bytes = A.offset ptr_shifted - A.offset ptr in
-  assert (offset_bytes = U32.v shift);
-  assert (offset_bytes = U32.v pos * U32.v size_class);
-  let offset_slot = offset_bytes / (U32.v size_class) in
-  lemma_div offset_bytes (U32.v pos) (U32.v size_class);
-  assert (offset_slot = U32.v pos);
-  let slot_as_pos = array_slot size_class arr slot_as_array in
-  assert (G.reveal slot_as_pos == offset_slot)
-
-let slab_vprop1 (size_class: sc) (arr: array U8.t{A.length arr = U32.v page_size})
-  (s: Seq.seq (r:nat{r < U32.v (nb_slots size_class)}))
-  : GTot (Seq.seq vprop)
-  =
-  let f = fun (k:nat{k < U32.v (nb_slots size_class)})
-    -> A.varray (slot_array size_class arr (U32.uint_to_t k)) in
-  Seq.map_seq_len f s;
-  let s' = Seq.map_seq f s in
-  s'
-
-let slab_vprop2 (size_class: sc) (arr: array U8.t{A.length arr = U32.v page_size})
-  (s: Seq.seq (r:nat{r < U32.v (nb_slots size_class)}))
-  : GTot (list vprop)
-  =
-  let s' = slab_vprop1 size_class arr s in
-  let r = Seq.seq_to_list s' in
-  r
-
-let slab_vprop3 (size_class: sc) (arr: array U8.t{A.length arr = U32.v page_size})
-  (s: Seq.seq (r:nat{r < U32.v (nb_slots size_class)}))
-  : GTot vprop
-  =
-  let r = slab_vprop2 size_class arr s in
-  starl r
-
-let slab_vprop2_lemma
-  (size_class: sc) (arr: array U8.t{A.length arr = U32.v page_size})
-  (s1 s2: Seq.seq (r:nat{r < U32.v (nb_slots size_class)}))
-  : Lemma
-  (slab_vprop2 size_class arr (Seq.append s1 s2)
-  == L.append (slab_vprop2 size_class arr s1) (slab_vprop2 size_class arr s2))
-  =
-  let f = fun (k:nat{k < U32.v (nb_slots size_class)})
-    -> A.varray (slot_array size_class arr (U32.uint_to_t k)) in
-  Seq.map_seq_append f s1 s2;
-  assert (
-     slab_vprop1 size_class arr (Seq.append s1 s2)
-  == Seq.append (slab_vprop1 size_class arr s1) (slab_vprop1 size_class arr s2));
-  lemma_seq_to_list_append
-    (slab_vprop1 size_class arr s1)
-    (slab_vprop1 size_class arr s2)
-
-let slab_vprop3_lemma
-  (size_class: sc) (arr: array U8.t{A.length arr = U32.v page_size})
-  (s1 s2: Seq.seq (r:nat{r < U32.v (nb_slots size_class)}))
-  : Lemma
-  (slab_vprop3 size_class arr (Seq.append s1 s2)
-  `equiv` (
-         (slab_vprop3 size_class arr s1)
-  `star` (slab_vprop3 size_class arr s2)))
-  =
-  let l1 = slab_vprop2 size_class arr s1 in
-  let l2 = slab_vprop2 size_class arr s2 in
-  slab_vprop2_lemma size_class arr s1 s2;
-  starl_append l1 l2
-
-let slab_vprop
-  (size_class: sc)
-  (arr: array U8.t{A.length arr = U32.v page_size})
-  (i:nat)
-  (j:nat{i <= j /\ j <= U32.v (nb_slots size_class)})
-  : Tot vprop
-  =
-  let s = Seq.slice (Seq.init (U32.v (nb_slots size_class)) (fun k -> k)) i j in
-  slab_vprop3 size_class arr s
-
-let slab_vprop_lemma
-  (size_class: sc)
-  (arr: array U8.t{A.length arr = U32.v page_size})
-  (i:nat)
-  (j:nat{i <= j /\ j <= U32.v (nb_slots size_class)})
-  (k:nat{i <= k /\ k <= j})
-  : Lemma
-  (slab_vprop size_class arr i j
-  `equiv` (
-         (slab_vprop size_class arr i k)
-  `star` (slab_vprop size_class arr k j)))
-  =
-  let s = Seq.init (U32.v (nb_slots size_class)) (fun k -> k) in
-  let s1 = Seq.slice s i j in
-  let s2, s3 = Seq.split s1 (k - i) in
-  Seq.lemma_split s1 (k - i);
-  assert (s2 == Seq.slice s1 0 (k - i));
-  Classical.forall_intro (lemma_index_slice s1 0 (k - i));
-  assert (s3 == Seq.slice s1 (k - i) (j - i));
-  Classical.forall_intro (lemma_index_slice s1 (k - i) (j - i));
-  slab_vprop3_lemma size_class arr s2 s3
-
-module SM = Steel.Memory
-
-let slab_vprop_sl_lemma
-  (size_class: sc)
-  (md: slab_metadata)
-  (arr: array U8.t{A.length arr = U32.v page_size})
-  (i:nat)
-  (j:nat{i <= j /\ j <= U32.v (nb_slots size_class)})
-  (k:nat{i <= k /\ k <= j})
-  (m: SM.mem)
-  : Lemma
-  (requires SM.interp (hp_of (
-    (slab_vprop size_class arr i j)
-  )) m)
-  (ensures SM.interp (hp_of (
-    (slab_vprop size_class arr i k `star`
-    slab_vprop size_class arr k j)
-  )) m)
-  =
-  slab_vprop_lemma size_class arr i j k;
-  let p = slab_vprop size_class arr i j in
-  let q = (slab_vprop size_class arr i k) `star`
-          (slab_vprop size_class arr k j) in
-  assert (p `equiv` q);
-  reveal_equiv p q;
-  assert (hp_of p `SM.equiv` hp_of q);
-  SM.reveal_equiv (hp_of p) (hp_of q)
-
-let slab_vprop_singleton_lemma
-  (size_class: sc)
-  (arr: array U8.t{A.length arr = U32.v page_size})
-  (pos: U32.t{0 <= (U32.v pos) /\ (U32.v pos) < U32.v (nb_slots size_class)})
-  : Lemma
-  (slab_vprop size_class arr (U32.v pos) (U32.v pos + 1)
-  ==
-  (A.varray (slot_array size_class arr pos) `star` emp)
-  )
-  =
-  let r = slab_vprop size_class arr (U32.v pos) (U32.v pos + 1) in
-  let s = Seq.slice (Seq.init (U32.v (nb_slots size_class)) (fun k -> k))
-    (U32.v pos) (U32.v pos + 1) in
-  assert (r == slab_vprop3 size_class arr s);
-  assert (r == starl (slab_vprop2 size_class arr s));
-  assert (r == starl (Seq.seq_to_list (slab_vprop1 size_class arr s)));
-  let f = fun (k:nat{k < U32.v (nb_slots size_class)})
-    -> A.varray (slot_array size_class arr (U32.uint_to_t k)) in
-  Seq.map_seq_len f s;
-  assert (Seq.length (slab_vprop1 size_class arr s) == 1);
-  Seq.map_seq_index f s 0;
-  assert (r == starl ([A.varray (slot_array size_class arr pos)]));
-  assert (r == A.varray (slot_array size_class arr pos) `star` emp)
-
 let allocate_slot_aux (#opened:_)
   (size_class: sc)
   (md: slab_metadata) (arr: array U8.t{A.length arr = U32.v page_size})
@@ -445,16 +222,6 @@ let allocate_slot_kiss (size_class: sc)
   //  (fun x y -> x == y)
   //  (fun _ -> ());
   return (G.hide (U32.v slot_pos), slot)
-
-assume val f (md: slab_metadata) : arr:array U8.t{A.length arr = U32.v page_size}
-
-
-[@@ __reduce__]
-unfold let p (size_class: sc)
-  =
-  fun (md: slab_metadata)
-  -> A.varray md
-     `star` slab_vprop size_class (f md) 0 (U32.v (nb_slots size_class))
 
 // Given a size class, return a free slot and update metadata
 // TODO: refine spec
@@ -568,7 +335,21 @@ let allocate_slab
   )
 
 // Given a size, return a size_class
-// TODO
+// TODO: improve max_sc bound
+// (requires an improved Steel while loop)
+let select_size_class (size: U32.t)
+  : Steel sc
+  emp (fun _ -> emp)
+  (requires fun _ -> U32.v size <= max_sc)
+  (ensures fun _ size_class _ -> U32.lte size size_class)
+  =
+  if U32.lte size 16ul then (
+    return 16ul
+  ) else if U32.lte size 32ul then (
+    return 32ul
+  ) else (
+    return 64ul
+  )
 
 (*)
 //noextract
