src/SizeClass.fst
@@ -1,0 +1,302 @@
+module SizeClass
+
+
+module U64 = FStar.UInt64
+module U32 = FStar.UInt32
+module U8 = FStar.UInt8
+
+open FStar.Ghost
+
+module SL = Selectors.LList
+open Steel.FractionalPermission
+module Mem = Steel.Memory
+open Steel.Effect.Atomic
+open Steel.Effect
+open Steel.Reference
+module SR = Steel.Reference
+module A = Steel.Array
+
+open Utils2
+open SlabsUtils
+
+assume val f (md: slab_metadata) : arr:array U8.t{A.length arr = U32.v page_size}
+
+[@@ __reduce__]
+unfold let p (size_class: sc)
+  =
+  fun (md: slab_metadata)
+  ->
+  (A.varray md `star`
+  slab_vprop size_class (f md) 0 (U32.v (nb_slots size_class)))
+
+[@@ __reduce__]
+unfold let p_empty (size_class: sc)
+  =
+  fun (md: slab_metadata)
+  ->
+  (A.varray md `vrefine`
+    (fun s ->
+      Seq.index s 0 = 0UL /\
+      Seq.index s 1 = 0UL /\
+      Seq.index s 2 = 0UL /\
+      Seq.index s 3 = 0UL))
+  `star`
+  slab_vprop size_class (f md) 0 (U32.v (nb_slots size_class))
+
+noeq
+type size_class_struct = {
+  size: sc;
+  partial_slabs: ref (SL.t slab_metadata);
+  empty_slabs: ref (SL.t slab_metadata);
+  region_start: array (arr:array U8.t{A.length arr = U32.v page_size});
+  lock: ref bool;
+  metadata_allocated: U32.t;
+}
+
+noeq
+type blob = {
+  scs_v: size_class_struct;
+  partial_slabs_v: SL.t slab_metadata;
+  empty_slabs_v: SL.t slab_metadata;
+}
+
+let size_class_sl'
+  (r: ref size_class_struct)
+  (blob: blob)
+  : Mem.slprop u#1
+  =
+  pts_to_sl r full_perm (blob.scs_v) `Mem.star`
+  pts_to_sl (blob.scs_v.partial_slabs) full_perm (blob.partial_slabs_v) `Mem.star`
+  //SL.ind_llist_sl (p_empty blob.scs_v.size) (blob.scs_v.empty_slabs)
+  pts_to_sl (blob.scs_v.empty_slabs) full_perm (blob.empty_slabs_v)
+
+let size_class_sl
+  (r: ref size_class_struct)
+  =
+  Mem.h_exists (size_class_sl' r)
+
+let size_class_sel_full'
+  (r: ref size_class_struct)
+  : selector' blob (size_class_sl r)
+  =
+  fun h ->
+    let b = Mem.id_elim_exists (size_class_sl' r) h in
+    b
+
+let size_class_sl'_witinv (r: ref size_class_struct)
+  : Lemma (Mem.is_witness_invariant (size_class_sl' r))
+  =
+  let aux (b1 b2: blob) (m: Mem.mem)
+  : Lemma
+  (requires
+    Mem.interp (size_class_sl' r b1) m /\
+    Mem.interp (size_class_sl' r b2) m
+  )
+  (ensures b1 == b2)
+  =
+  pts_to_witinv r full_perm;
+  assert (b1.scs_v == b2.scs_v);
+  pts_to_witinv (b1.scs_v.partial_slabs) full_perm;
+  pts_to_witinv (b1.scs_v.empty_slabs) full_perm
+  in
+  Classical.forall_intro_3 (Classical.move_requires_3 aux)
+
+let size_class_sel_depends_only_on
+  (r: ref size_class_struct)
+  (m0:Mem.hmem (size_class_sl r)) (m1:Mem.mem{Mem.disjoint m0 m1})
+  : Lemma
+  (size_class_sel_full' r m0 == size_class_sel_full' r (Mem.join m0 m1))
+  =
+  let m' = Mem.join m0 m1 in
+  let b1 = reveal (Mem.id_elim_exists (size_class_sl' r) m0) in
+  let b2 = reveal (Mem.id_elim_exists (size_class_sl' r) m') in
+  size_class_sl'_witinv r;
+  Mem.elim_wi (size_class_sl' r) b1 b2 m'
+
+let size_class_sel_depends_only_on_core
+  (r: ref size_class_struct)
+  (m0:Mem.hmem (size_class_sl r))
+  : Lemma
+  (size_class_sel_full' r m0 == size_class_sel_full' r (Mem.core_mem m0))
+  =
+  let b1 = reveal (Mem.id_elim_exists (size_class_sl' r) m0) in
+  let b2 = reveal (Mem.id_elim_exists (size_class_sl' r) (Mem.core_mem m0)) in
+  size_class_sl'_witinv r;
+  Mem.elim_wi (size_class_sl' r) b1 b2 (Mem.core_mem m0)
+
+let size_class_sel (r: ref size_class_struct)
+  : selector blob (size_class_sl r)
+  =
+  Classical.forall_intro_2 (size_class_sel_depends_only_on r);
+  Classical.forall_intro (size_class_sel_depends_only_on_core r);
+  size_class_sel_full' r
+
+[@@ __steel_reduce__]
+let size_class_full' (r: ref size_class_struct) : vprop'
+  = {
+    hp = size_class_sl r;
+    t = blob;
+    sel = size_class_sel r;
+  }
+unfold
+let size_class_full (r: ref size_class_struct) = VUnit (size_class_full' r)
+
+[@@ __steel_reduce__]
+let v_sc_full (#p: vprop) (r: ref size_class_struct)
+  (h: rmem p{FStar.Tactics.with_tactic selector_tactic (can_be_split p (size_class_full r) /\ True)})
+  = h (size_class_full r)
+
+let unpack_sc_lemma
+  (r: ref size_class_struct)
+  (b: blob)
+  (m: Mem.mem)
+  : Lemma
+  (requires
+    Mem.interp (size_class_sl r) m /\
+    size_class_sel r m == b
+  )
+  (ensures (
+    Mem.interp (
+      SR.ptr r `Mem.star`
+      SR.ptr (b.scs_v.partial_slabs) `Mem.star`
+      SR.ptr (b.scs_v.empty_slabs)
+    ) m /\
+    sel_of (vptr r) m == b.scs_v /\
+    sel_of (vptr b.scs_v.partial_slabs) m == b.partial_slabs_v /\
+    sel_of (vptr b.scs_v.empty_slabs) m == b.empty_slabs_v
+  ))
+  =
+  let p1 = pts_to_sl r full_perm b.scs_v in
+  let p2 = pts_to_sl (b.scs_v.partial_slabs) full_perm (b.partial_slabs_v) in
+  let p3 = pts_to_sl (b.scs_v.empty_slabs) full_perm (b.empty_slabs_v) in
+  let sl = p1 `Mem.star` p2 `Mem.star` p3 in
+  assert (Mem.interp sl m);
+
+  let m12, m3 = Mem.id_elim_star (p1 `Mem.star` p2) p3 m in
+  let m1, m2 = Mem.id_elim_star p1 p2 m12 in
+  // #1
+  intro_ptr_interp r b.scs_v m1;
+  ptr_sel_interp r m1;
+  pts_to_witinv r full_perm;
+  // #2
+  intro_ptr_interp (b.scs_v.partial_slabs) (b.partial_slabs_v) m2;
+  ptr_sel_interp (b.scs_v.partial_slabs) m2;
+  pts_to_witinv (b.scs_v.partial_slabs) full_perm;
+  // #3
+  intro_ptr_interp (b.scs_v.empty_slabs) (b.empty_slabs_v) m3;
+  ptr_sel_interp (b.scs_v.empty_slabs) m3;
+  pts_to_witinv (b.scs_v.empty_slabs) full_perm;
+  Mem.intro_star
+    (SR.ptr r)
+    (SR.ptr (b.scs_v.partial_slabs)) m1 m2;
+  assert (reveal m12 == Mem.join m1 m2);
+  Mem.intro_star
+    (SR.ptr r `Mem.star` SR.ptr (b.scs_v.partial_slabs))
+    (SR.ptr (b.scs_v.empty_slabs)) m12 m3;
+  assert (m == Mem.join m12 m3);
+  //@2
+  admit ()
+
+
+let unpack_sc (r: ref size_class_struct)
+  : Steel size_class_struct
+  (size_class_full r)
+  (fun scs ->
+    vptr r `star`
+    vptr scs.partial_slabs `star`
+    vptr scs.empty_slabs
+  )
+  (requires fun _ -> True)
+  (ensures fun h0 scs h1 ->
+    let b = v_sc_full r h0 in
+    sel r h1 == scs /\
+    True
+    //@2 b.scs_v.partial_slabs == sel scs.partial_slabs h1 /\
+    //@2 b.scs_v.empty_slabs == sel scs.empty_slabs h1
+  )
+  =
+  let h = get () in
+  let b = hide (v_sc_full r h) in
+  change_slprop
+    (size_class_full r)
+    (vptr r `star`
+    vptr b.scs_v.partial_slabs `star`
+    vptr b.scs_v.empty_slabs)
+    b
+    ((b.scs_v, b.partial_slabs_v), b.empty_slabs_v)
+    (fun m -> unpack_sc_lemma r (reveal b) m);
+  let scs = read r in
+  change_slprop_rel
+    (vptr b.scs_v.partial_slabs)
+    (vptr scs.partial_slabs)
+    (fun x y -> x == y)
+    (fun _ -> ());
+  change_slprop_rel
+    (vptr b.scs_v.empty_slabs)
+    (vptr scs.empty_slabs)
+    (fun x y -> x == y)
+    (fun _ -> ());
+  return scs
+
+let pack_sc_lemma
+  (r: ref size_class_struct)
+  (b: blob)
+  (m: Mem.mem)
+  : Lemma
+  (requires
+    Mem.interp (
+      SR.ptr r `Mem.star`
+      SR.ptr (b.scs_v.partial_slabs) `Mem.star`
+      SR.ptr (b.scs_v.empty_slabs)
+    ) m /\
+    sel_of (vptr r) m == b.scs_v /\
+    sel_of (vptr b.scs_v.partial_slabs) m == b.partial_slabs_v /\
+    sel_of (vptr b.scs_v.empty_slabs) m == b.empty_slabs_v
+  )
+  (ensures (
+    Mem.interp (size_class_sl r) m /\
+    size_class_sel r m == b
+  ))
+  =
+  admit ()
+
+let pack_sc (#opened:_)
+  (r: ref size_class_struct)
+  (scs: size_class_struct)
+  : SteelGhost unit opened
+  (vptr r `star`
+  vptr scs.partial_slabs `star`
+  vptr scs.empty_slabs)
+  (fun _ -> size_class_full r)
+  (requires fun h0 -> sel r h0 == scs)
+  (ensures fun _ _ _ ->
+    //@2
+    True)
+  =
+  let h0 = get () in
+  let b : erased blob = hide ({
+    scs_v = scs;
+    partial_slabs_v = sel scs.partial_slabs h0;
+    empty_slabs_v = sel scs.empty_slabs h0;
+  }) in
+  change_slprop
+    (vptr r `star`
+    vptr b.scs_v.partial_slabs `star`
+    vptr b.scs_v.empty_slabs)
+    (size_class_full r)
+    ((b.scs_v, b.partial_slabs_v), b.empty_slabs_v)
+    b
+    (fun m -> pack_sc_lemma r (reveal b) m)
+
+// TODO
+// - intermediate step with lemmas in order to have packing/unpacking
+// @2- vptr -> llist: which predicate ?
+
+let temp (r1 r2: ref size_class_struct)
+  : SteelT U32.t
+  (size_class_full r1)
+  (fun _ -> size_class_full r1)
+  =
+  let scs = unpack_sc r1 in
+  pack_sc r1 scs;
+  return 0ul
