src/SlabsUtils.fst
@@ -1,0 +1,215 @@
+module SlabsUtils
+
+module U64 = FStar.UInt64
+module U32 = FStar.UInt32
+module U8 = FStar.UInt8
+
+module G = FStar.Ghost
+module L = FStar.List.Tot
+open FStar.Mul
+
+open Steel.Effect.Atomic
+open Steel.Effect
+open Steel.Reference
+//module SR = Steel.Reference
+module A = Steel.Array
+
+
+open Utils
+open Utils2
+
+#push-options "--z3rlimit 20"
+let slot_array (size_class: sc) (arr: array U8.t) (pos: U32.t)
+  : Pure (array U8.t)
+  (requires
+    U32.v pos < U32.v (nb_slots size_class) /\
+    A.length arr = U32.v page_size)
+  (ensures fun r ->
+    A.length r = U32.v size_class /\
+    same_base_array r arr /\
+    True)
+  =
+  let ptr = A.ptr_of arr in
+  let shift = U32.mul pos size_class in
+  assert (U32.v shift < A.length arr);
+  let ptr_shifted = A.ptr_shift ptr shift in
+  (| ptr_shifted, G.hide (U32.v size_class) |)
+#pop-options
+
+let array_slot (size_class: sc) (arr: array U8.t) (slot: array U8.t)
+  : Pure (G.erased int)
+  (requires same_base_array arr slot)
+  (ensures fun r -> True)
+  =
+  let ptr1 = A.ptr_of arr in
+  assert (A.offset ptr1 <= A.base_len (A.base ptr1));
+  let ptr2 = A.ptr_of slot in
+  assert (A.offset ptr2 <= A.base_len (A.base ptr2));
+  let offset_bytes = A.offset ptr2 - A.offset ptr1 in
+  let offset_slot = offset_bytes / (U32.v size_class) in
+  offset_slot
+
+let array_slot_slot_array_bij (size_class: sc) (arr: array U8.t) (pos: U32.t)
+  : Lemma
+  (requires
+    U32.v pos < U32.v (nb_slots size_class) /\
+    A.length arr = U32.v page_size)
+  (ensures (
+    let slot_as_array = slot_array size_class arr pos in
+    let slot_as_pos = array_slot size_class arr slot_as_array in
+    G.reveal slot_as_pos = U32.v pos))
+  =
+  let ptr = A.ptr_of arr in
+  let shift = U32.mul pos size_class in
+  assert (U32.v shift < A.length arr);
+  let ptr_shifted = A.ptr_shift ptr shift in
+  let slot_as_array = slot_array size_class arr pos in
+  assert (A.ptr_of slot_as_array == ptr_shifted);
+  let offset_bytes = A.offset ptr_shifted - A.offset ptr in
+  assert (offset_bytes = U32.v shift);
+  assert (offset_bytes = U32.v pos * U32.v size_class);
+  let offset_slot = offset_bytes / (U32.v size_class) in
+  lemma_div offset_bytes (U32.v pos) (U32.v size_class);
+  assert (offset_slot = U32.v pos);
+  let slot_as_pos = array_slot size_class arr slot_as_array in
+  assert (G.reveal slot_as_pos == offset_slot)
+
+let slab_vprop1 (size_class: sc) (arr: array U8.t{A.length arr = U32.v page_size})
+  (s: Seq.seq (r:nat{r < U32.v (nb_slots size_class)}))
+  : GTot (Seq.seq vprop)
+  =
+  let f = fun (k:nat{k < U32.v (nb_slots size_class)})
+    -> A.varray (slot_array size_class arr (U32.uint_to_t k)) in
+  Seq.map_seq_len f s;
+  let s' = Seq.map_seq f s in
+  s'
+
+let slab_vprop2 (size_class: sc) (arr: array U8.t{A.length arr = U32.v page_size})
+  (s: Seq.seq (r:nat{r < U32.v (nb_slots size_class)}))
+  : GTot (list vprop)
+  =
+  let s' = slab_vprop1 size_class arr s in
+  let r = Seq.seq_to_list s' in
+  r
+
+let slab_vprop3 (size_class: sc) (arr: array U8.t{A.length arr = U32.v page_size})
+  (s: Seq.seq (r:nat{r < U32.v (nb_slots size_class)}))
+  : GTot vprop
+  =
+  let r = slab_vprop2 size_class arr s in
+  starl r
+
+let slab_vprop2_lemma
+  (size_class: sc) (arr: array U8.t{A.length arr = U32.v page_size})
+  (s1 s2: Seq.seq (r:nat{r < U32.v (nb_slots size_class)}))
+  : Lemma
+  (slab_vprop2 size_class arr (Seq.append s1 s2)
+  == L.append (slab_vprop2 size_class arr s1) (slab_vprop2 size_class arr s2))
+  =
+  let f = fun (k:nat{k < U32.v (nb_slots size_class)})
+    -> A.varray (slot_array size_class arr (U32.uint_to_t k)) in
+  Seq.map_seq_append f s1 s2;
+  assert (
+     slab_vprop1 size_class arr (Seq.append s1 s2)
+  == Seq.append (slab_vprop1 size_class arr s1) (slab_vprop1 size_class arr s2));
+  lemma_seq_to_list_append
+    (slab_vprop1 size_class arr s1)
+    (slab_vprop1 size_class arr s2)
+
+let slab_vprop3_lemma
+  (size_class: sc) (arr: array U8.t{A.length arr = U32.v page_size})
+  (s1 s2: Seq.seq (r:nat{r < U32.v (nb_slots size_class)}))
+  : Lemma
+  (slab_vprop3 size_class arr (Seq.append s1 s2)
+  `equiv` (
+         (slab_vprop3 size_class arr s1)
+  `star` (slab_vprop3 size_class arr s2)))
+  =
+  let l1 = slab_vprop2 size_class arr s1 in
+  let l2 = slab_vprop2 size_class arr s2 in
+  slab_vprop2_lemma size_class arr s1 s2;
+  starl_append l1 l2
+
+let slab_vprop
+  (size_class: sc)
+  (arr: array U8.t{A.length arr = U32.v page_size})
+  (i:nat)
+  (j:nat{i <= j /\ j <= U32.v (nb_slots size_class)})
+  : Tot vprop
+  =
+  let s = Seq.slice (Seq.init (U32.v (nb_slots size_class)) (fun k -> k)) i j in
+  slab_vprop3 size_class arr s
+
+let slab_vprop_lemma
+  (size_class: sc)
+  (arr: array U8.t{A.length arr = U32.v page_size})
+  (i:nat)
+  (j:nat{i <= j /\ j <= U32.v (nb_slots size_class)})
+  (k:nat{i <= k /\ k <= j})
+  : Lemma
+  (slab_vprop size_class arr i j
+  `equiv` (
+         (slab_vprop size_class arr i k)
+  `star` (slab_vprop size_class arr k j)))
+  =
+  let s = Seq.init (U32.v (nb_slots size_class)) (fun k -> k) in
+  let s1 = Seq.slice s i j in
+  let s2, s3 = Seq.split s1 (k - i) in
+  Seq.lemma_split s1 (k - i);
+  assert (s2 == Seq.slice s1 0 (k - i));
+  Classical.forall_intro (lemma_index_slice s1 0 (k - i));
+  assert (s3 == Seq.slice s1 (k - i) (j - i));
+  Classical.forall_intro (lemma_index_slice s1 (k - i) (j - i));
+  slab_vprop3_lemma size_class arr s2 s3
+
+module SM = Steel.Memory
+
+let slab_vprop_sl_lemma
+  (size_class: sc)
+  (md: slab_metadata)
+  (arr: array U8.t{A.length arr = U32.v page_size})
+  (i:nat)
+  (j:nat{i <= j /\ j <= U32.v (nb_slots size_class)})
+  (k:nat{i <= k /\ k <= j})
+  (m: SM.mem)
+  : Lemma
+  (requires SM.interp (hp_of (
+    (slab_vprop size_class arr i j)
+  )) m)
+  (ensures SM.interp (hp_of (
+    (slab_vprop size_class arr i k `star`
+    slab_vprop size_class arr k j)
+  )) m)
+  =
+  slab_vprop_lemma size_class arr i j k;
+  let p = slab_vprop size_class arr i j in
+  let q = (slab_vprop size_class arr i k) `star`
+          (slab_vprop size_class arr k j) in
+  assert (p `equiv` q);
+  reveal_equiv p q;
+  assert (hp_of p `SM.equiv` hp_of q);
+  SM.reveal_equiv (hp_of p) (hp_of q)
+
+let slab_vprop_singleton_lemma
+  (size_class: sc)
+  (arr: array U8.t{A.length arr = U32.v page_size})
+  (pos: U32.t{0 <= (U32.v pos) /\ (U32.v pos) < U32.v (nb_slots size_class)})
+  : Lemma
+  (slab_vprop size_class arr (U32.v pos) (U32.v pos + 1)
+  ==
+  (A.varray (slot_array size_class arr pos) `star` emp)
+  )
+  =
+  let r = slab_vprop size_class arr (U32.v pos) (U32.v pos + 1) in
+  let s = Seq.slice (Seq.init (U32.v (nb_slots size_class)) (fun k -> k))
+    (U32.v pos) (U32.v pos + 1) in
+  assert (r == slab_vprop3 size_class arr s);
+  assert (r == starl (slab_vprop2 size_class arr s));
+  assert (r == starl (Seq.seq_to_list (slab_vprop1 size_class arr s)));
+  let f = fun (k:nat{k < U32.v (nb_slots size_class)})
+    -> A.varray (slot_array size_class arr (U32.uint_to_t k)) in
+  Seq.map_seq_len f s;
+  assert (Seq.length (slab_vprop1 size_class arr s) == 1);
+  Seq.map_seq_index f s 0;
+  assert (r == starl ([A.varray (slot_array size_class arr pos)]));
+  assert (r == A.varray (slot_array size_class arr pos) `star` emp)
