src/Utils2.fsti
@@ -1,0 +1,41 @@
+module Utils2
+
+module U64 = FStar.UInt64
+module U32 = FStar.UInt32
+
+open Steel.Effect.Atomic
+open Steel.Effect
+open Steel.Reference
+module A = Steel.Array
+
+
+let array = Steel.ST.Array.array
+let ptr = Steel.ST.Array.ptr
+
+unfold let slab_metadata = r:array U64.t{A.length r = 4}
+
+//TODO: should not be hardcoded
+let page_size = 4096ul
+let slab_max_number = 4096ul
+
+noextract
+let min_sc = 16
+noextract
+let max_sc = 64
+
+//TODO: second constraint should be relaxed
+//currently does not support size classes with <64 slots
+//that require a subtle loop to read only possible
+//corresponding slots in the bitmap
+let sc = x:U32.t{min_sc <= U32.v x /\ U32.v x <= max_sc}
+
+
+let nb_slots (size_class: sc)
+  : Pure U32.t
+  (requires True)
+  (ensures fun r ->
+    U32.v r >= 1 /\
+    U32.v r <= 256
+  )
+  =
+  U32.div page_size size_class
